sepref seq

theories/Compositional_Structures/Basic_Modules/Component_Types/Electoral_Module_Ref.thy
@@ -1,8 +1,7 @@
 theory Electoral_Module_Ref                      
-  imports "Verified_Voting_Rule_Construction.Profile_List"
+  imports "Social_Choice_Types/Profile_List_Monadic"
           "Social_Choice_Types/Ballot_Refinement"
           "Verified_Voting_Rule_Construction.Electoral_Module"
-           Refine_Imperative_HOL.IICF
          
 begin                            
 
@@ -36,6 +35,35 @@ abbreviation "result_assn \<equiv> alts_assn \<times>\<^sub>a
                               alts_assn \<times>\<^sub>a
                                alts_assn"
 
+definition elect_monadic ::
+  "'a Electoral_Module_Ref \<Rightarrow> 'a set \<Rightarrow> 'a  Profile_List \<Rightarrow> 'a set nres" where
+  "elect_monadic m A p \<equiv> do {
+    result <- m A p;
+    RETURN (elect_r result)
+  }"
+
+definition defer_monadic ::
+  "'a Electoral_Module_Ref \<Rightarrow> 'a set \<Rightarrow> 'a  Profile_List \<Rightarrow> 'a set nres" where
+  "defer_monadic m A p \<equiv> do {
+    result <- m A p;
+    RETURN (defer_r result)
+  }"
+
+definition reject_monadic ::
+  "'a Electoral_Module_Ref \<Rightarrow> 'a set \<Rightarrow> 'a  Profile_List \<Rightarrow> 'a set nres" where
+  "reject_monadic m A p \<equiv> do {
+    result <- m A p;
+    RETURN (reject_r result)
+  }"
+
+
+lemma elect_check_correct:
+shows "(elect_monadic, (\<lambda> e A p. SPEC (\<lambda> rem. rem = (elect e A p)))) \<in> 
+    em_rel \<rightarrow> \<langle>Id\<rangle>alt_set_rel \<rightarrow> profile_rel \<rightarrow> \<langle>\<langle>Id\<rangle>alt_set_rel\<rangle>nres_rel"
+  apply (refine_rcg)
+  unfolding elect_monadic_def em_rel_def
+  apply clarify
+  oops
 
 locale sepref_access =
   fixes mod1 :: "nat Electoral_Module_Ref"
@@ -50,55 +78,42 @@ begin
 
   lemma this_loc: "sepref_access mod1 mod1_impl" by unfold_locales
 
-definition elect_ref ::
-  "nat set \<Rightarrow> nat Profile_List \<Rightarrow> nat set nres" where
-  "elect_ref A p \<equiv> do {
-    result <- mod1 A p;
-    RETURN (elect_r result)}
-  "
-
-lemma elect_monadic_refine:
-  fixes em:: "nat Electoral_Module"
-  assumes "(mod1,(\<lambda> A p. SPEC (\<lambda> rem. rem = em A p))) \<in> elec_mod_relb"
-  shows "(elect_ref, (\<lambda> A p. SPEC (\<lambda> rem. rem = (elect em A p)))) \<in> 
-    \<langle>nat_rel\<rangle>alt_set_rel \<rightarrow> profile_rel \<rightarrow> \<langle>\<langle>nat_rel\<rangle>alt_set_rel\<rangle>nres_rel"
-  unfolding elect_ref_def
-proof (refine_vcg, rename_tac A' A pl pr)
-   fix A' A:: "nat set"
-  fix pl :: "nat Profile_List"
-  fix pr :: "nat Profile"
-  assume arel: "(A', A) \<in> \<langle>nat_rel\<rangle>alt_set_rel"
-  assume prel: " (pl, pr) \<in> profile_rel"
-  from arel have aeq: "A' = A" by (auto simp add: alt_set_rel_def in_br_conv)
-  from arel have fina: "finite A'" by (auto simp add: alt_set_rel_def in_br_conv)
-  note assms[THEN fun_relD,THEN fun_relD, THEN nres_relD, where x2 = A' and x'2 = A
-      and x1 = pl and x'1 = pr]
-  from this have "  mod1 A' pl
-  \<le>  (SPEC (\<lambda>rem. rem = em A pr)) " using refine_IdD prod_rel_id set_rel_id
-    using arel prel by fastforce  
-  from this arel prel  show " mod1 A' pl \<bind> (\<lambda>result. RETURN (elect_r result))
-       \<le> \<Down> (\<langle>nat_rel\<rangle>alt_set_rel) (SPEC (\<lambda>rem. rem = elect em A pr))"
-    using specify_left
-    sorry
-qed
-  
-
 
 sepref_register "mod1" :: "nat Electoral_Module_Ref"
 
 declare mod1_impl [sepref_fr_rules]
 
 schematic_goal elect_impl:
-  "(uncurry ?c, uncurry elect_ref) \<in> (alts_set_impl_assn)\<^sup>k *\<^sub>a profile_impl_assn\<^sup>k \<rightarrow>\<^sub>a alts_set_impl_assn"
-  unfolding elect_ref_def
+  "(uncurry ?c, uncurry (elect_monadic mod1)) \<in> (alts_set_impl_assn)\<^sup>k *\<^sub>a profile_impl_assn\<^sup>k \<rightarrow>\<^sub>a alts_set_impl_assn"
+  unfolding elect_monadic_def
   by sepref
 
 concrete_definition (in -) elect_sep uses sepref_access.elect_impl
   prepare_code_thms (in -) elect_sep_def
-  lemmas elect_impl_refine = elect_sep.refine[OF this_loc]
+lemmas elect_impl_refine = elect_sep.refine[OF this_loc]
+
+schematic_goal defer_impl:
+  "(uncurry ?c, uncurry (defer_monadic mod1)) \<in> (alts_set_impl_assn)\<^sup>k *\<^sub>a profile_impl_assn\<^sup>k \<rightarrow>\<^sub>a alts_set_impl_assn"
+  unfolding defer_monadic_def
+  by sepref
+
+concrete_definition (in -) defer_sep uses sepref_access.defer_impl
+  prepare_code_thms (in -) defer_sep_def
+  lemmas defer_impl_refine = defer_sep.refine[OF this_loc]
+
+schematic_goal reject_impl:
+  "(uncurry ?c, uncurry (reject_monadic mod1)) \<in> (alts_set_impl_assn)\<^sup>k *\<^sub>a profile_impl_assn\<^sup>k \<rightarrow>\<^sub>a alts_set_impl_assn"
+  unfolding reject_monadic_def
+  by sepref
+
+concrete_definition (in -) reject_sep uses sepref_access.reject_impl
+  prepare_code_thms (in -) reject_sep_def
+  lemmas reject_impl_refine = reject_sep.refine[OF this_loc]
+
 
 end
 
-term "sepref_access.elect_ref"
+thm "elect_sep_def"
+thm "elect_sep.refine"
 
 end
