theories/Compositional_Structures/Sequential_Composition_Ref.thy
@@ -1,0 +1,205 @@
+theory Sequential_Composition_Ref
+  imports "Basic_Modules/Component_Types/Electoral_Module_Ref"
+        "Verified_Voting_Rule_Construction.Sequential_Composition"
+begin
+
+definition sequential_composition_mon :: "'a Electoral_Module_Ref \<Rightarrow> 'a Electoral_Module_Ref \<Rightarrow>
+        'a Electoral_Module_Ref" where
+"sequential_composition_mon m n A p = do {
+      let electm = elect_monadic m;
+      let electn = elect_monadic n;
+      let rejectm = reject_monadic m;
+      let rejectn = reject_monadic n;
+      let defm = defer_monadic m;
+      let defn = defer_monadic n;
+    
+      new_A <- defm A p;
+      new_p <- limit_profile_l new_A p;
+      
+      electmA <- electm A p;
+      electnA' <- electn new_A new_p;
+      rejectmA <- rejectm A p;
+      rejectnA' <- rejectn new_A new_p;
+      def <- defn new_A new_p;
+ 
+      RETURN (rejectmA,rejectmA,electmA)}"
+
+(*      let elec = electmA \<union> electnA';
+      let rej = rejectmA \<union> rejectnA';
+*)
+
+locale seqcomp_impl =
+  fixes m :: "nat Electoral_Module_Ref"
+  fixes m_impl :: "(nat, unit) hashtable
+      \<Rightarrow> (nat array \<times> nat) list
+         \<Rightarrow> ((nat, unit) hashtable \<times> (nat, unit) hashtable \<times> (nat, unit) hashtable) Heap"
+  fixes n :: "nat Electoral_Module_Ref"
+  fixes n_impl :: "(nat, unit) hashtable
+      \<Rightarrow> (nat array \<times> nat) list
+         \<Rightarrow> ((nat, unit) hashtable \<times> (nat, unit) hashtable \<times> (nat, unit) hashtable) Heap"
+  assumes 
+    m_impl: "(uncurry m_impl, uncurry m)
+        \<in> (alts_set_impl_assn)\<^sup>k *\<^sub>a profile_impl_assn\<^sup>k \<rightarrow>\<^sub>a result_impl_assn"  
+    and
+    n_impl: "(uncurry n_impl, uncurry n)
+        \<in> (alts_set_impl_assn)\<^sup>k *\<^sub>a profile_impl_assn\<^sup>k \<rightarrow>\<^sub>a result_impl_assn"
+
+begin
+
+  lemma this_loc: "seqcomp_impl m m_impl n n_impl" by unfold_locales
+
+(*lemma [sepref_import_param]: "(limit_profile_l,limit_profile_l)
+ \<in> \<langle>Id\<rangle>alt_set_rel \<rightarrow> \<langle>\<langle>Id\<rangle>list_rel\<rangle>list_rel \<rightarrow> \<langle>\<langle>\<langle>Id\<rangle>list_rel\<rangle>list_rel\<rangle>nres_rel"
+  unfolding limit_profile_l.simps limit_monadic_def
+  apply (auto)
+proof (rename_tac A' A p)
+   fix A' A :: "'a set"
+  fix p :: "'a Profile_List"
+  assume arel: "(A', A) \<in> \<langle>Id\<rangle>alt_set_rel"
+  from arel have aeq: "A' = A" by (simp add: alt_set_rel_def in_br_conv)
+  show "(nfoldli p (\<lambda>_. True)
+         (\<lambda>x np.
+             WHILE\<^sub>T\<^bsup>limit_monadic_inv A' x\<^esup> (\<lambda>(i, nbal). i < length x)
+              (\<lambda>(i, nbal).
+                  ASSERT (i < length x) \<bind>
+                  (\<lambda>_. let c = x ! i
+                        in RETURN (if c \<in> A' then (i + 1, nbal @ [c]) else (i + 1, nbal))))
+              (0, []) \<bind>
+             (\<lambda>x. (case x of (i, x) \<Rightarrow> RETURN x) \<bind> (\<lambda>newb. RETURN (np @ [newb]))))
+         [],
+        nfoldli p (\<lambda>_. True)
+         (\<lambda>x np.
+             WHILE\<^sub>T\<^bsup>limit_monadic_inv A x\<^esup> (\<lambda>(i, nbal). i < length x)
+              (\<lambda>(i, nbal).
+                  ASSERT (i < length x) \<bind>
+                  (\<lambda>_. let c = x ! i
+                        in RETURN (if c \<in> A then (i + 1, nbal @ [c]) else (i + 1, nbal))))
+              (0, []) \<bind>
+             (\<lambda>x. (case x of (i, x) \<Rightarrow> RETURN x) \<bind> (\<lambda>newb. RETURN (np @ [newb]))))
+         [])
+       \<in> \<langle>Id\<rangle>nres_rel"
+  apply (refine_vcg)
+   apply refine_dref_type
+    by (auto simp add: aeq)
+qed
+
+lemma [sepref_import_param]: "(defer_monadic,defer_monadic)
+  \<in>   (\<langle>Id\<rangle>alt_set_rel \<rightarrow> \<langle>\<langle>Id\<rangle>list_rel\<rangle>list_rel 
+  \<rightarrow> \<langle>\<langle>Id\<rangle>set_rel \<times>\<^sub>r \<langle>Id\<rangle>set_rel \<times>\<^sub>r \<langle>Id\<rangle>set_rel\<rangle>nres_rel)
+   \<rightarrow> \<langle>Id\<rangle>alt_set_rel \<rightarrow> \<langle>\<langle>Id\<rangle>list_rel\<rangle>list_rel \<rightarrow> \<langle>\<langle>Id\<rangle>set_rel\<rangle>nres_rel"
+  unfolding  defer_monadic_def
+   apply (auto)
+  apply (rename_tac em' em A' A p)
+  apply refine_vcg
+   apply refine_dref_type
+   apply auto
+proof -
+  fix em' em :: "'a Electoral_Module_Ref"
+  fix A' A :: "'a set"
+  fix p :: "'a Profile_List"
+  assume em_id: "(em', em) \<in> \<langle>Id\<rangle>alt_set_rel \<rightarrow> Id \<rightarrow> \<langle>Id\<rangle>nres_rel"
+  assume arel: "(A', A) \<in> \<langle>Id\<rangle>alt_set_rel"
+  from this have aeq: "A' = A" by (simp add: in_br_conv alt_set_rel_def)
+  from em_id[THEN fun_relD, THEN fun_relD, THEN nres_relD, THEN refine_IdD] arel
+  show "em' A' p \<le> em A p"
+    by blast
+qed
+
+ lemma [sepref_import_param]: "(elect_monadic,elect_monadic)
+  \<in>   (\<langle>Id\<rangle>alt_set_rel \<rightarrow> \<langle>\<langle>Id\<rangle>list_rel\<rangle>list_rel 
+  \<rightarrow> \<langle>\<langle>Id\<rangle>set_rel \<times>\<^sub>r \<langle>Id\<rangle>set_rel \<times>\<^sub>r \<langle>Id\<rangle>set_rel\<rangle>nres_rel)
+   \<rightarrow> \<langle>Id\<rangle>alt_set_rel \<rightarrow> \<langle>\<langle>Id\<rangle>list_rel\<rangle>list_rel \<rightarrow> \<langle>\<langle>Id\<rangle>set_rel\<rangle>nres_rel"
+  unfolding  elect_monadic_def
+   apply (auto)
+  apply (rename_tac em' em A' A p)
+  apply refine_vcg
+   apply refine_dref_type
+   apply auto
+proof -
+  fix em' em :: "'a Electoral_Module_Ref"
+  fix A' A :: "'a set"
+  fix p :: "'a Profile_List"
+  assume em_id: "(em', em) \<in> \<langle>Id\<rangle>alt_set_rel \<rightarrow> Id \<rightarrow> \<langle>Id\<rangle>nres_rel"
+  assume arel: "(A', A) \<in> \<langle>Id\<rangle>alt_set_rel"
+  from this have aeq: "A' = A" by (simp add: in_br_conv alt_set_rel_def)
+  from em_id[THEN fun_relD, THEN fun_relD, THEN nres_relD, THEN refine_IdD] arel
+  show "em' A' p \<le> em A p"
+    by blast
+qed
+
+ lemma [sepref_import_param]: "(reject_monadic,reject_monadic)
+  \<in>   (\<langle>Id\<rangle>alt_set_rel \<rightarrow> \<langle>\<langle>Id\<rangle>list_rel\<rangle>list_rel 
+  \<rightarrow> \<langle>\<langle>Id\<rangle>set_rel \<times>\<^sub>r \<langle>Id\<rangle>set_rel \<times>\<^sub>r \<langle>Id\<rangle>set_rel\<rangle>nres_rel)
+   \<rightarrow> \<langle>Id\<rangle>alt_set_rel \<rightarrow> \<langle>\<langle>Id\<rangle>list_rel\<rangle>list_rel \<rightarrow> \<langle>\<langle>Id\<rangle>set_rel\<rangle>nres_rel"
+  unfolding  reject_monadic_def
+   apply (auto)
+  apply (rename_tac em' em A' A p)
+  apply refine_vcg
+   apply refine_dref_type
+   apply auto
+proof -
+  fix em' em :: "'a Electoral_Module_Ref"
+  fix A' A :: "'a set"
+  fix p :: "'a Profile_List"
+  assume em_id: "(em', em) \<in> \<langle>Id\<rangle>alt_set_rel \<rightarrow> Id \<rightarrow> \<langle>Id\<rangle>nres_rel"
+  assume arel: "(A', A) \<in> \<langle>Id\<rangle>alt_set_rel"
+  from this have aeq: "A' = A" by (simp add: in_br_conv alt_set_rel_def)
+  from em_id[THEN fun_relD, THEN fun_relD, THEN nres_relD, THEN refine_IdD] arel
+  show "em' A' p \<le> em A p"
+    by blast
+qed*)
+  
+
+sepref_register "m" :: "nat Electoral_Module_Ref"
+sepref_register "n" :: "nat Electoral_Module_Ref"
+
+thm n_impl
+
+declare m_impl [sepref_fr_rules]
+declare n_impl [sepref_fr_rules]
+
+sepref_definition electm_imp is
+  "(uncurry (elect_monadic m))" 
+    :: "(alts_set_impl_assn)\<^sup>k *\<^sub>a profile_impl_assn\<^sup>k \<rightarrow>\<^sub>a alts_set_impl_assn"
+  unfolding elect_monadic_def
+  by sepref
+
+schematic_goal electn_imp:
+  "(uncurry ?c, uncurry (elect_monadic n)) \<in> (alts_set_impl_assn)\<^sup>k *\<^sub>a profile_impl_assn\<^sup>k \<rightarrow>\<^sub>a alts_set_impl_assn"
+  unfolding elect_monadic_def
+  by sepref
+
+definition seqt :: 
+   "nat Electoral_Module_Ref" where
+"seqt A p = do {
+     electmA <- (elect_monadic m) A p;
+     RETURN(electmA,op_hs_empty,op_hs_empty)
+}"
+
+lemma val: shows "sepref_access m m_impl"
+  using m_impl by unfold_locales
+
+lemma elecmsep:
+  shows" (uncurry
+ (\<lambda>ai bi.
+     m_impl ai bi \<bind> (\<lambda>x'. return (fst x'))) ,
+ uncurry (elect_monadic m))
+\<in> (hs.assn nat_assn)\<^sup>k *\<^sub>a
+   profile_impl_assn\<^sup>k \<rightarrow>\<^sub>a hs.assn nat_assn"
+  using val elect_sep_def elect_sep.refine
+  by auto
+
+declare elecmsep [sepref_fr_rules]
+
+sepref_definition seqt_imp is
+  "(uncurry (seqt))" 
+    :: "alts_set_impl_assn\<^sup>k *\<^sub>a profile_impl_assn\<^sup>k \<rightarrow>\<^sub>a result_impl_assn"
+  unfolding seqt_def 
+  apply sepref_dbg_keep
+
+
+end
+
+
+
+end
